Need to change syntactic judgments

mechanization/theories/Core/Soundness/Extension/SystemAnnotated.v
@@ -9,93 +9,480 @@ Import Syntax_Notations.
 Reserved Notation "⊫ Γ > sts " (in custom judg at level 80, Γ custom exp, sts constr).
 Reserved Notation "Γ : sts ⊫ M : A > s" (in custom judg at level 80, Γ custom exp, sts constr, M custom exp, A custom exp, s constr).
 Reserved Notation "Γ : sts ⊫ A > s" (in custom judg at level 80, Γ custom exp, sts constr, A custom exp, s constr).
-Reserved Notation "Γ : sts ⊫s σ : Δ > sts'" (in custom judg at level 80, Γ custom exp, sts constr, σ custom exp, Δ custom exp, sts' constr).
+Reserved Notation "Γ : stsΓ ⊫s σ : Δ > stsΔ" (in custom judg at level 80, Γ custom exp, stsΓ constr, σ custom exp, Δ custom exp, stsΔ constr).
+(* Reserved Notation "'#' x : A > s ∈ Γ : sts" (in custom judg at level 80, x constr at level 0, A custom exp, s constr, Γ custom exp at level 50, sts constr). *)
 
 Generalizable All Variables.
 
+(* Inductive ctx_lookup_ann {P} : nat -> typ P -> P -> ctx P -> list P -> Prop :=  *)
+(* | here_a : `({{ #0 : A > s ∈ Γ, A : s :: sts }} ) *)
+(* | there_a : `({{ #n : A > s ∈ Γ : sts }} -> {{ #(S n) : A[Wk] > s ∈ Γ, B : (sb :: sts) }}) *)
+(* where "'#' x : A > s ∈ Γ : sts" := (ctx_lookup_ann x A s Γ sts) (in custom judg) : type_scope. *)
+  
 Inductive wf_ctx_ann {P} : ctx P -> list P -> Prop :=
 | wfa_ctx_empty : {{ ⊫ ⋅ > nil }}
 | wfa_ctx_extend :
   `( {{ ⊫ Γ > sts }} ->
-     {{ Γ ⊢ A : Sort@s }} ->
+     {{ Γ : sts ⊫ A : Sort@s > s' }} ->
      {{ ⊫ Γ, A > (s :: sts) }} )
-where "⊫ Γ > sts" := (wf_ctx_ann Γ sts) (in custom judg) : type_scope.
+where "⊫ Γ > sts" := (wf_ctx_ann Γ sts) (in custom judg) : type_scope
 
-#[export]
-Hint Constructors wf_ctx_ann : mcpts.
-
-Lemma wf_ctx_then_wf_ctx_ann {P} : forall {Γ : ctx P},
-    {{ ⊢ Γ }} ->
-    exists sts, {{ ⊫ Γ > sts }}.
-Proof.
-  induction 1; mauto 2.
-  destruct_conjs.
-  eexists; mauto 2.
-Qed.
-
-Lemma wf_ctx_ann_then_wf_ctx {P} : forall {Γ : ctx P} {sts},
-    {{ ⊫ Γ > sts }} ->
-    {{ ⊢ Γ }}.
-Proof.
-  induction 1; mauto 2.
-Qed.
-
-
-Inductive wf_exp_ann {P} : ctx P -> list P -> exp P -> exp P -> P -> Prop :=
-| wf_st :
+with wf_exp_ann {P} : ctx P -> list P -> exp P -> P -> exp P -> Prop :=
+| wfa_st :
   `( Ax P s1 s2 -> Ax P s2 s3 ->
      {{ ⊫ Γ > sts }} ->
      {{ Γ : sts ⊫ Sort@s1 : Sort@s2 > s3 }} )
-| wf_pi :
+(** Functions *)
+| wfa_pi :
   `( forall (r : Ru P s1 s2 s3),
         Ax P s3 s3' ->
         {{ Γ : sts ⊫ A : Sort@s1 > s1' }} ->
         {{ Γ, A : (s1 :: sts) ⊫ B : Sort@s2 > s2' }} ->
         {{ Γ : sts ⊫ Π r A B : Sort@s3 > s3' }} )
-where "Γ : sts ⊫ M : A > s" := (wf_exp_ann Γ sts M A s) (in custom judg) : type_scope.
+| wfa_fn :
+  `( forall (r : Ru P s1 s2 s3),
+        {{ Γ : sts ⊫ A : Sort@s1 > s1' }} ->
+        {{ Γ, A : (s1 :: sts) ⊫ B : Sort@s2 > s2' }} ->
+        {{ Γ, A : (s1 :: sts) ⊫ M : B > s2 }} ->
+        {{ Γ : sts ⊫ λ r A M : Π r A B > s3 }} )
+| wfa_app :
+  `( forall (r : Ru P s1 s2 s3),
+        {{ Γ : sts ⊫ A : Sort@s1 > s1' }} ->
+        {{ Γ, A : (s1 :: sts) ⊫ B : Sort@s2 > s2' }} ->
+        {{ Γ : sts ⊫ M : Π r A B > s3 }} ->
+        {{ Γ : sts ⊫ N : A > s1 }} ->
+        {{ Γ : sts ⊫ M N : B[Id,,N] > s2 }} )
+   
+| wfa_vlookup :
+  `( {{ ⊫ Γ > sts }} ->
+     {{ #x : A ∈ Γ }} ->
+     {{ Γ : sts ⊫ A > s }} ->
+     {{ Γ : sts ⊫ #x : A > s }} )
+   
+(** Naturals *)
+| wfa_nat :
+  `( forall (r : Ru_nat P sn),
+        Ax P sn sn' ->
+        {{ ⊫ Γ > sts }} ->
+        {{ Γ : sts ⊫ ℕ : Sort@sn > sn' }} )
+| wfa_zero :
+  `( forall (r : Ru_nat P sn),
+        {{ ⊫ Γ > sts }} ->
+        {{ Γ : sts ⊫ zero : ℕ > sn }} )
+| wfa_succ :
+  `( forall (r : Ru_nat P sn),
+        {{ Γ : sts ⊫ M : ℕ > sn' }} ->
+        {{ Γ : sts ⊫ succ M : ℕ > sn }} )
+| wfa_rec :
+  `( forall (r : Ru_nat P sn),
+        {{ Γ, ℕ : (sn :: sts) ⊫ A : Sort@sa > sa' }} ->
+        {{ Γ : sts ⊫ MZ : A[Id,,zero] > sa }} ->
+        {{ Γ, ℕ, A : (sa :: (sn :: sts)) ⊫ MS : A[Wk∘Wk,,succ #1] > sa }} ->
+        {{ Γ : sts ⊫ M : ℕ > sn }} ->
+        {{ Γ : sts ⊫ rec M return A | zero -> MZ | succ -> MS end : A[Id,,M] > sa }} )
 
-Lemma wf_exp_ann_implies_wf_exp {P} : forall {Γ : ctx P} {sts M A s},
+| wfa_exp_sub :
+  `( {{ Γ : sts ⊫s σ : Δ > sts' }} ->
+     {{ Δ : sts' ⊫ M : A > s }} ->
+     {{ Γ : sts ⊫ M[σ] : A[σ] > s }} )
+
+| wfa_exp_conv :
+  `( {{ Γ : sts ⊫ M : A > s }} ->
+     {{ Γ ⊢ A ≈ A' }} ->
+     {{ Γ : sts ⊫ M : A' > s }} )
+| wfa_exp_conv_st :
+  `( {{ Γ : sts ⊫ M : A > s }} ->
+     {{ Γ : sts ⊫ A > s' }} ->
+     {{ Γ : sts ⊫ M : A > s' }} )
+where "Γ : sts ⊫ M : A > s" := (wf_exp_ann Γ sts A s M) (in custom judg) : type_scope
+
+with wf_typ_ann {P} : ctx P -> list P -> typ P -> P -> Prop :=
+| wfa_typ_st :
+  `( Ax P s s' ->
+     {{ ⊫ Γ > sts }} ->
+     {{ Γ : sts ⊫ Sort@s > s' }} )
+| wfa_typ_exp :
+  `( {{ Γ : sts ⊫ A : Sort@s > s' }} ->
+     {{ Γ : sts ⊫ A > s }} )
+| wfa_typ_clo :
+  `( {{ Γ : sts ⊫s σ : Δ > sts' }} ->
+     {{ Δ : sts' ⊫ A > s }} ->
+     {{ Γ : sts ⊫ A[σ] > s }} )
+where "Γ : sts ⊫ A > s" := (wf_typ_ann Γ sts A s) (in custom judg) : type_scope
+                                                                             
+with wf_sub_ann {P} : ctx P -> list P -> ctx P -> list P -> sub P -> Prop :=
+| wfa_sub_id :
+  `( {{ ⊫ Γ > sts }} ->
+     {{ Γ : sts ⊫s Id : Γ > sts }} )
+| wfa_sub_weaken :
+  `( {{ ⊫ Γ, A > s :: sts }} ->
+     {{ Γ, A : s :: sts ⊫s Wk : Γ > sts }} )
+| wfa_sub_compose :
+  `( {{ Γ1 : sts1 ⊫s σ2 : Γ2 > sts2 }} ->
+     {{ Γ2 : sts2 ⊫s σ1 : Γ3 > sts3 }} ->
+     {{ Γ1 : sts1 ⊫s σ1∘σ2 : Γ3 > sts3 }} )
+| wfa_sub_extend :
+  `( {{ Γ : stsΓ ⊫s σ : Δ > stsΔ }} ->
+     {{ Δ : stsΔ ⊫ A : Sort@s > s' }} ->
+     {{ Γ : stsΓ ⊫ M : A[σ] > s }} ->
+     {{ Γ : stsΓ ⊫s σ,,M : Δ, A > s :: stsΔ }} )
+| wfa_sub_conv :
+  `( {{ Γ : stsΓ ⊫s σ : Δ > stsΔ }} ->
+     {{ ⊫ Δ' > stsΔ' }} ->
+     {{ ⊢ Δ ≈ Δ' }} ->
+     {{ Γ : stsΓ ⊫s σ : Δ' > stsΔ' }} )
+| wfa_sub_conv_sts :
+  `( {{ Γ : stsΓ ⊫s σ : Δ > stsΔ }} ->
+     {{ ⊫ Δ > stsΔ' }} ->
+     {{ Γ : stsΓ ⊫s σ : Δ > stsΔ' }} )
+where "Γ : stsΓ ⊫s σ : Δ > stsΔ" := (wf_sub_ann Γ stsΓ Δ stsΔ σ) (in custom judg) : type_scope.
+
+#[export]
+Hint Constructors wf_ctx_ann wf_exp_ann wf_typ_ann wf_sub_ann : mcpts.
+
+Scheme wf_ctx_ann_mut_ind := Induction for wf_ctx_ann Sort Prop
+with wf_exp_ann_mut_ind := Induction for wf_exp_ann Sort Prop
+with wf_sub_ann_mut_ind := Induction for wf_sub_ann Sort Prop.                                          
+Combined Scheme syntactic_wf_ann_mut_ind from
+  wf_ctx_ann_mut_ind,
+  wf_exp_ann_mut_ind,
+  wf_sub_ann_mut_ind.
+
+
+#[local]
+Ltac gen_irrel_IH P full_P exp_irrel typ_irrel sub_irrel H :=
+  match type of H with
+  | {{ ^?Γ : ?sts ⊫ ^?M : ^?A > ?s }} =>
+      let IH := fresh "IHwf_exp_ann" in
+      pose proof exp_irrel P full_P Γ sts M A s H as IH
+  | {{ ^?Γ : ?sts ⊫ ^?A > ?s }} =>
+      let IH := fresh "IHwf_typ_ann" in
+      pose proof typ_irrel P full_P Γ sts A s H as IH 
+  | {{ ^?Γ : ?stsΓ ⊫s ^?σ : ^?Δ > ?stsΔ }} =>
+      let Hσ := fresh "IHwf_sub_ann" in
+      pose proof sub_irrel P full_P Γ stsΓ σ Δ stsΔ H as Hσ
+  end.
+
+#[local]
+Ltac specialize_IHs :=
+  match goal with
+  | IH : forall sts', {{ ⊫ ^?Γ > sts' }} -> {{ ^?Γ : sts' ⊫ ^?M : ^?A > ?s }},
+    HΓ : {{ ⊫ ^?Γ > ?sts' }} |- _ => specialize (IH _ HΓ)
+  | IH : forall sts', {{ ⊫ ^?Γ > sts' }} -> {{ ^?Γ : sts' ⊫ ^?A > ?s }},
+    HΓ : {{ ⊫ ^?Γ > ?sts' }} |- _ => specialize (IH _ HΓ)
+  | IH : forall sts', {{ ⊫ ^?Γ > sts' }} -> {{ ^?Γ : sts' ⊫s ^?σ : ^?Δ > ?stsΔ }},
+    HΓ : {{ ⊫ ^?Γ > ?sts' }} |- _ => specialize (IH _ HΓ)
+end.
+
+  
+Lemma wf_exp_sts_irrel {P} (full_P : FullSig P) : forall {Γ : ctx P} {sts} {M A s},
     {{ Γ : sts ⊫ M : A > s }} ->
-    {{ Γ ⊢ M : A }}.
+    forall sts', {{ ⊫ Γ > sts' }} ->
+            {{ Γ : sts' ⊫ M : A > s }}
+
+with wf_typ_sts_irrel {P} (full_P : FullSig P) : forall {Γ : ctx P} {sts} {A s},
+    {{ Γ : sts ⊫ A > s }} ->
+    forall sts', {{ ⊫ Γ > sts' }} ->
+            {{ Γ : sts' ⊫ A > s }}
+              
+with wf_sub_sts_irrel {P} (full_P : FullSig P) : forall {Γ : ctx P} {stsΓ σ Δ stsΔ},
+    {{ Γ : stsΓ ⊫s σ : Δ > stsΔ }} ->
+    forall stsΓ', {{ ⊫ Γ > stsΓ' }} ->
+             {{ Γ : stsΓ' ⊫s σ : Δ > stsΔ }}.
 Proof.
-  induction 1;
-    match goal with
-    | H : {{ ⊫ ^?Γ > ?sts }} |- _ =>
-        assert {{ ⊢ Γ }} by (eapply (wf_ctx_ann_then_wf_ctx H))
-    | _ => idtac
-    end;
-    mauto 2.  
+  all: (inversion_clear 1;
+        (on_all_hyp: gen_irrel_IH P full_P wf_exp_sts_irrel wf_typ_sts_irrel wf_sub_sts_irrel);
+        clear wf_exp_sts_irrel wf_typ_sts_irrel wf_sub_sts_irrel;
+        intros stsΓ' HΓ);
+    try specialize_IHs;
+    only 2-4: (assert {{ ⊫ Γ,A0 > s1 :: stsΓ' }} as HΓA by mauto 2);
+    only 9: (assert (exists sn', Ax P sn sn') as [sn'] by (eapply full_P);
+             assert {{ Γ : stsΓ' ⊫ ℕ : Sort@sn > sn' }} by mauto 2;
+             assert {{ ⊫ Γ, ℕ > sn :: stsΓ' }} by mauto 2;
+             try specialize_IHs;
+             assert {{ ⊫ Γ, ℕ, A0 > s :: sn :: stsΓ' }} by mauto 2
+            );
+    only 12: (specialize_IHs);
+    only 17: (inversion_clear HΓ);
+    try solve [econstructor; mauto 2].
+
+  inversion_clear H0.
+  assert {{ Δ, A : s0 :: sts ⊫s Wk : Δ > sts }} by mauto 3.
+  eapply wfa_sub_conv_sts; mauto 2.
 Qed.
 
-Lemma wf_exp_implies_wf_exp_ann_helper {P} (full_P : FullSig P) : forall {Γ : ctx P} {sts M A},
-    {{ Γ ⊢ M : A }} ->
-    {{ ⊫ Γ > sts }} ->
-    exists s,
-      {{ Γ : sts ⊫ M : A > s }}.
+  
+#[local]
+Ltac gen_ann_presup_IH P exp_presup typ_presup sub_presup H :=
+  match type of H with
+  | {{ ^?Γ : ?sts ⊫ ^?M : ^?A > ?s }} =>
+      let HM := fresh "HM" in
+      pose proof exp_presup _ _ _ _ _ _ H as HM
+  | {{ ^?Γ : ?sts ⊫ ^?A > ?s }} =>
+      let HA := fresh "HA" in
+      pose proof typ_presup _ _ _ _ _ H as HM
+  | {{ ^?Γ : ?sts ⊫s ^?σ : ^?Δ > ?sts' }} =>
+      let Hσ := fresh "Hσ" in
+      pose proof sub_presup _ _ _ _ _ _ H as Hσ
+  end.
+  
+Lemma wf_exp_ann_ctx_presup {P} : forall {Γ : ctx P} {sts M A s},
+    {{ Γ : sts ⊫ M : A > s }} ->
+    {{ ⊫ Γ > sts }}
+
+with wf_typ_ann_ctx_presup {P} : forall {Γ : ctx P} {sts A s},
+    {{ Γ : sts ⊫ A > s }} ->
+    {{ ⊫ Γ > sts }}
+      
+with wf_sub_ann_ctx_presup {P} : forall {Γ : ctx P} {sts σ Δ sts'},
+    {{ Γ : sts ⊫s σ : Δ > sts' }} ->
+    {{ ⊫ Γ > sts }}.
 Proof.
-  intros * H.
-  gen sts.
-  induction H.
-  - intros.
+  all: inversion_clear 1;
+    (on_all_hyp: gen_ann_presup_IH P wf_exp_ann_ctx_presup wf_typ_ann_ctx_presup wf_sub_ann_ctx_presup);
+    clear wf_exp_ann_ctx_presup wf_typ_ann_ctx_presup wf_sub_ann_ctx_presup;
+    mauto 2.
+Qed.
+
+
+Lemma wf_sub_ann_domain_presup {P} : forall {Γ : ctx P} {sts σ Δ sts'},
+    {{ Γ : sts ⊫s σ : Δ > sts' }} ->
+    {{ ⊫ Δ > sts' }}.
+Proof.
+  induction 1; mauto 2.
+  inversion_clear H; eassumption.
+Qed.  
+
+#[local]
+Ltac gen_annotated_judg_IH P full_P ann_ctx ann_exp ann_typ ann_sub H :=
+  match type of H with
+  | {{ ⊢ ^?Γ }} =>
+      let HΓ := fresh "HΓ" in
+      pose proof ann_ctx P full_P Γ H as HΓ
+  | {{ ^?Γ ⊢ ^?M : ^?A }} =>
+      let HM := fresh "HM" in
+      pose proof ann_exp P full_P Γ M A H as HM
+  | {{ ^?Γ ⊢ ^?A }} =>
+      let HA := fresh "HA" in
+      pose proof ann_typ P full_P Γ A H as HA
+  | {{ ^?Γ ⊢s ^?σ : ^?Δ }} =>
+      let Hσ := fresh "Hσ" in
+      pose proof ann_sub P full_P Γ σ Δ H as Hσ
+  end.
+
+Lemma wf_ctx_implies_wf_ctx_ann {P} (full_P : FullSig P) : forall {Γ : ctx P},
+    {{ ⊢ Γ }} ->
+    exists sts, {{ ⊫ Γ > sts }}
+
+with wf_exp_implies_wf_exp_ann {P} (full_P : FullSig P) : forall {Γ : ctx P} {M A},
+    {{ Γ ⊢ M : A }} ->
+    exists sts s, {{ Γ : sts ⊫ M : A > s }}
+
+with wf_typ_implies_wf_typ_ann {P} (full_P : FullSig P) : forall {Γ : ctx P} {A},
+    {{ Γ ⊢ A }} ->
+    exists sts s, {{ Γ : sts ⊫ A > s }}
+               
+with wf_sub_implies_wf_sub_ann {P} (full_P : FullSig P) : forall {Γ : ctx P} {σ Δ},
+    {{ Γ ⊢s σ : Δ }} ->
+    exists sts sts', {{ Γ : sts ⊫s σ : Δ > sts' }}.
+Proof.
+  all: inversion_clear 1;
+    (on_all_hyp: gen_annotated_judg_IH P full_P wf_ctx_implies_wf_ctx_ann wf_exp_implies_wf_exp_ann wf_typ_implies_wf_typ_ann wf_sub_implies_wf_sub_ann);
+    clear wf_ctx_implies_wf_ctx_ann wf_exp_implies_wf_exp_ann wf_typ_implies_wf_typ_ann wf_sub_implies_wf_sub_ann;
+    mauto 3.
+  
+  - destruct HM as [sts [s' HA]].
+    destruct HΓ as [sts' HΓ].
+    assert {{ Γ0 : sts' ⊫ A : Sort@s > s' }} by (eapply wf_exp_sts_irrel; mauto 2).
+    eexists; mauto 2.
+  - destruct HΓ as [sts HΓ].
     assert (exists s3, Ax P s2 s3) as [s3] by (eapply full_P).
-    eexists; econstructor; mauto 2.
-
-  - intros.
-    assert (exists s1', {{ Γ : sts ⊫ A : Sort@s1 > s1' }}) as [s1'] by mauto 2.
-    assert {{ ⊫ Γ, A > (s1 :: sts) }} by mauto 2.
-    assert (exists s2', {{ Γ, A : (s1 :: sts) ⊫ B : Sort@s2 > s2' }}) as [s2'] by mauto 2.
+    do 2 eexists; mauto 2.
+  - destruct HM0 as [sts [s1' HA]].
+    destruct HM as [sts' [s2' HB]].
+    assert {{ ⊫ Γ > sts }} by (eapply wf_exp_ann_ctx_presup; mauto 2).
+    assert {{ ⊫ Γ, A0 > s1 :: sts }} by mauto 2.
+    assert {{ Γ, A0 : (s1 :: sts) ⊫ B : Sort@s2 > s2' }} by (eapply wf_exp_sts_irrel; mauto 2).
     assert (exists s3', Ax P s3 s3') as [s3'] by (eapply full_P).
-    eexists; econstructor; mauto 2.
-Admitted.
+    do 2 eexists; mauto 2.
+  - destruct HM1 as [stsΓ [s1' HA0]].
+    destruct HM0 as [stsΓA0 [s2' HB]].
+    destruct HM as [stsΓA0' [sb HM0]].
+    assert {{ ⊫ Γ > stsΓ }} by (eapply wf_exp_ann_ctx_presup; mauto 2).
+    assert {{ ⊫ Γ, A0 > s1 :: stsΓ }} by mauto 2.
+    assert {{ Γ, A0 : s1 :: stsΓ ⊫ B : Sort@s2 > s2' }} by (eapply wf_exp_sts_irrel; mauto 2).
+    assert {{ Γ, A0 : s1 :: stsΓ ⊫ B > s2 }} by mauto 2.
+    assert {{ Γ, A0 : s1 :: stsΓ ⊫ M0 : B > sb }} by (eapply wf_exp_sts_irrel; mauto 2).
+    assert {{ Γ, A0 : s1 :: stsΓ ⊫ M0 : B > s2 }} by (eapply wfa_exp_conv_st; mauto 2).
+    do 2 eexists; mauto 2.
+  - destruct HM as [sts [sa0 HN]].
+    assert {{ ⊫ Γ > sts }} as HΓ by (eapply wf_exp_ann_ctx_presup; mauto 2).
 
-Lemma wf_exp_implies_wf_exp_ann {P} (full_P : FullSig P) : forall {Γ : ctx P} {M A},
-    {{ Γ ⊢ M : A }} ->
-    exists sts s,
-      {{ Γ : sts ⊫ M : A > s }}.
-Proof.
-  intros * H.
-  gen_presup H.
-  assert (exists sts, {{ ⊫ Γ > sts }}) as [sts] by (eapply wf_ctx_then_wf_ctx_ann; mauto 2).
-  eexists.
-  eapply wf_exp_implies_wf_exp_ann_helper; mauto 2.
+    destruct HM2 as [sts'' [s1' HA0]].
+    assert {{ Γ : sts ⊫ A0 : Sort@s1 > s1' }} by (eapply wf_exp_sts_irrel; mauto 2).
+    clear HA0; rename H into HA0.
+
+    assert {{ Γ : sts ⊫ A0 > s1 }} as HA0s1 by mauto 2.
+    assert {{ Γ : sts ⊫ N : A0 > s1 }} by mauto 2.
+    clear HN; rename H into HN.
+    
+    destruct HM1 as [stsΓA0 [s2' HB]].
+    assert {{ ⊫ Γ, A0 > s1 :: sts }} as HΓA by mauto 2.
+    assert {{ Γ, A0 : s1 :: sts ⊫ B : Sort@s2 > s2' }} by (eapply wf_exp_sts_irrel; mauto 2).
+    clear HB; rename H into HB.
+    
+    destruct HM0 as [sts' [sΠ HM0]].
+    assert {{ Γ : sts ⊫ M0 : Π r A0 B > sΠ }} by (eapply wf_exp_sts_irrel; mauto 2).
+    clear HM0; rename H into HM0.
+    assert {{ Γ : sts ⊫ Π r A0 B > s3 }} as HΠ.
+    {
+      assert (exists s3', Ax P s3 s3') as [s3'] by (eapply full_P).
+      mauto 3.
+    }
+    assert {{ Γ : sts ⊫ M0 : Π r A0 B > s3 }} by mauto 3.
+    clear HM0; rename H into HM0.
+    
+    do 2 eexists; mauto 2.
+    
+  - destruct HΓ as [sts HΓ].
+    assert (exists s, {{ Γ ⊢ A : Sort@s }}) as [s] by mauto 2.
+    do 2 eexists; mauto 2.
+    
+  - destruct HΓ as [sts HΓ].
+    assert (exists s', Ax P s s') as [s'] by (eapply full_P).
+    do 2 eexists; mauto 2.
+  - destruct HΓ as [sts HΓ].
+    do 2 eexists; mauto 2.
+  - destruct HM as [sts [s' HM0]].
+    do 2 eexists; mauto 2.
+  - rename s into sn.
+    rename s' into s.
+    assert (exists sn', Ax P sn sn') as [sn'] by (eapply full_P).
+    destruct HM1 as [stsΓ [sa HMZ]].
+    assert {{ ⊫ Γ > stsΓ }} by (eapply wf_exp_ann_ctx_presup; mauto 2).
+    assert {{ Γ : stsΓ ⊫ ℕ : Sort@sn > sn' }} by mauto 2.
+    assert {{ ⊫ Γ, ℕ > sn :: stsΓ }} by mauto 2.
+    
+    destruct HM2 as [stsΓℕ [s' HA0]].
+    assert {{ Γ, ℕ : sn :: stsΓ ⊫ A0 : Sort@s > s' }} by (eapply wf_exp_sts_irrel; mauto 2).
+    clear HA0; rename H7 into HA0.
+
+    assert {{ Γ, ℕ : sn :: stsΓ ⊫ A0 > s }} by mauto 2.
+    assert {{ ⊫ Γ, ℕ, A0 > s :: sn :: stsΓ }} by mauto 2.
+    assert {{ Γ : stsΓ ⊫ MZ : A0[Id,,zero] > s }}.
+    {
+      enough {{ Γ : stsΓ ⊫ A0[Id,,zero] > s }} by mauto 3.
+      eapply wfa_typ_clo; mauto 2.
+      econstructor; mauto 2.
+      econstructor; mauto 2.
+      econstructor; mauto 2.
+      symmetry.
+      econstructor; mauto 3.
+    }
+    clear HMZ; rename H0 into HMZ.
+    clear sa.
+    
+    destruct HM0 as [stsΓℕA0 [sa HMS]].
+    assert {{ Γ, ℕ, A0 : s :: sn :: stsΓ ⊫ MS : A0[Wk∘Wk,,succ #1] > s }}.
+    {
+      assert {{ Γ, ℕ, A0 : s :: sn :: stsΓ ⊫ MS : A0[Wk∘Wk,,succ #1] > sa }} by (eapply wf_exp_sts_irrel; mauto 2).
+      enough {{ Γ, ℕ, A0 : s :: sn :: stsΓ ⊫ A0[Wk∘Wk,,succ #1] > s }} by mauto 3.
+      eapply wfa_typ_clo; mauto 2.
+      econstructor; mauto 4.
+      gen_presup H2.
+      assert {{ Γ, ℕ, A0 ⊢s Wk∘Wk : Γ }} by (econstructor; mauto 3).
+      assert {{ Γ, ℕ, A0 ⊢ ℕ[Wk∘Wk] ≈ ℕ : Sort@sn }} by (econstructor; mauto 2).
+      assert {{ Γ, ℕ, A0 ⊢ ℕ[Wk∘Wk] ≈ ℕ[Wk][Wk] : Sort@sn }}.
+      {
+        eapply wf_exp_eq_conv' with (A := {{{ Sort@sn[Wk∘Wk] }}}); mauto 3.
+        eapply wf_exp_eq_sub_compose; econstructor; mauto 2.
+      }
+      assert {{ Γ, ℕ, A0 ⊢ ℕ[Wk][Wk] ≈ ℕ : Sort@sn }} by (etransitivity; mauto 2).
+      eapply wfa_exp_conv with (A := {{{ ℕ }}}); mauto 2.
+      - eapply wfa_succ; [eapply r|].
+        eapply wfa_exp_conv with (A := {{{ ℕ[Wk][Wk] }}}); mauto 2.
+        econstructor; mauto 3.
+        eapply wf_conv with (A := {{{ Sort@sn[Wk][Wk] }}}); mauto 2.
+        + econstructor; mauto 2.
+          econstructor; econstructor; mauto 2.
+        + transitivity {{{ Sort@sn[Wk∘Wk] }}}; [symmetry|]; econstructor; mauto 2.
+          eapply wf_exp_eq_conv' with (A := {{{ Sort@sn'[Wk∘Wk] }}}); mauto 3.
+          eapply wf_exp_eq_sub_compose; econstructor; mauto 2.
+      - symmetry; mauto 3.
+    }
+    clear HMS; rename H0 into HMS.
+
+    destruct HM as [stsΓ' [sn'' HM0]].
+    assert {{ Γ : stsΓ ⊫ M0 : ℕ > sn }}.
+    {
+      assert {{ Γ : stsΓ ⊫ M0 : ℕ > sn'' }} by (eapply wf_exp_sts_irrel; mauto 2).
+      assert {{ Γ : stsΓ ⊫ ℕ > sn }} by mauto 2.
+      mauto 2.
+    }
+    clear HM0; rename H0 into HM0.
+
+    do 2 eexists; mauto 2.
+    
+  - destruct HM as [sts [s HA0]].
+    destruct Hσ as [stsΓ [stsΔ Hσ]].
+    assert {{ ⊫ Δ > stsΔ }} by (eapply wf_sub_ann_domain_presup; mauto 2).
+    assert {{ Δ : stsΔ ⊫ M0 : A0 > s }} by (eapply wf_exp_sts_irrel; mauto 2).
+    do 2 eexists; mauto 2.    
+  - destruct HM as [sts [s HM]].
+    do 2 eexists; mauto 2.
+  - destruct HΓ as [sts HΓ].
+    assert (exists s', Ax P s s') as [s'] by (eapply full_P).
+    do 2 eexists; mauto 2.
+  - destruct HM as [sts [s' HA]].
+    do 2 eexists; mauto 2.
+  - destruct HA as [stsΔ [s HA0]].
+    destruct Hσ as [stsΓ [stsΔ' Hσ]].
+    assert {{ ⊫ Δ > stsΔ' }} by (eapply wf_sub_ann_domain_presup; mauto 2).
+    assert {{ Δ : stsΔ' ⊫ A0 > s }} by (eapply wf_typ_sts_irrel; mauto 2).
+    do 2 eexists; mauto 2.
+  - destruct HΓ as [sts HΔ].
+    do 2 eexists; mauto 2.
+  - destruct HΓ as [sts HΔA].
+    inversion_clear HΔA.
+    assert {{ ⊫ Δ, A > s :: sts0 }} by mauto 2.
+    do 2 eexists; mauto 2.
+  - destruct Hσ as [stsΓ2 [stsΔ Hσ1]].
+    destruct Hσ0 as [stsΓ [stsΓ2' Hσ2]].
+    assert {{ ⊫ Γ2 > stsΓ2' }} by (eapply wf_sub_ann_domain_presup; mauto 2).
+    assert {{ Γ2 : stsΓ2' ⊫s σ1 : Δ > stsΔ }} by (eapply wf_sub_sts_irrel; mauto 2).
+    do 2 eexists; mauto 2.
+  - destruct HM as [stsΓ [sa HM]].
+    destruct HM0 as [stsΔ0 [s' HA]].
+    destruct Hσ as [stsΓ' [stsΔ0' Hσ0]].
+    assert {{ ⊫ Δ0 > stsΔ0' }} by (eapply wf_sub_ann_domain_presup; mauto 2).
+    assert {{ Δ0 : stsΔ0' ⊫ A : Sort@s > s' }} by (eapply wf_exp_sts_irrel; mauto 2).
+    assert {{ ⊫ Γ > stsΓ' }} by (eapply wf_exp_ann_ctx_presup; mauto 2).
+    assert {{ Γ : stsΓ' ⊫ M : A[σ0] > sa }} by (eapply wf_exp_sts_irrel; mauto 2).
+    assert {{ Δ0 : stsΔ0' ⊫ A > s }} by mauto 2.
+    assert {{ Γ : stsΓ' ⊫ M : A[σ0] > s }} by mauto 3.    
+    do 2 eexists; mauto 2.
+    
+  - destruct HΓ as [sts HΔ].
+    destruct Hσ as [stsΓ [stsΔ0 Hσ]].
+    do 2 eexists; mauto 2.
 Qed.
+
+Lemma wf_judg_ann_implies_wf_judg {P} :
+  (forall (Γ : ctx P) sts, {{ ⊫ Γ > sts }} -> {{ ⊢ Γ }}) /\
+    (forall (Γ : ctx P) sts A s M, {{ Γ : sts ⊫ M : A > s }} -> {{ Γ ⊢ M : A }}) /\
+    (forall (Γ : ctx P) sts Δ sts' σ, {{ Γ : sts ⊫s σ : Δ > sts' }} -> {{ Γ ⊢s σ : Δ }}).
+Proof.
+  eapply syntactic_wf_ann_mut_ind; mauto 2.
+Qed.
+
+Corollary wf_ctx_ann_implies_wf_ctx {P} : forall {Γ : ctx P} {sts},
+    {{ ⊫ Γ > sts }} -> {{ ⊢ Γ }}.
+Proof. intros; eapply wf_judg_ann_implies_wf_judg; mauto 2. Qed.
+
+Corollary wf_exp_ann_implies_wf_exp {P} : forall {Γ : ctx P} {sts A s M},
+    {{ Γ : sts ⊫ M : A > s }} -> {{ Γ ⊢ M : A }}.
+Proof. intros; eapply wf_judg_ann_implies_wf_judg; mauto 2. Qed.
+
+Corollary wf_sub_ann_implies_wf_sub {P} : forall {Γ : ctx P} {sts Δ sts' σ},
+    {{ Γ : sts ⊫s σ : Δ > sts' }} -> {{ Γ ⊢s σ : Δ }}.
+Proof. intros; eapply wf_judg_ann_implies_wf_judg; mauto 2. Qed.
