mechanization/theories/Core/Soundness/Realizability.v
@@ -31,7 +31,7 @@ Lemma var_arith {P} : forall (Γ1 Γ2 : ctx P) (A : typ P),
     length (Γ1 ++ A :: Γ2) - length Γ2 - 1 = length Γ1.
 Proof.
   intros.
-  rewrite List.length_app. simpl.
+  rewrite List.app_length. simpl.
   lia.
 Qed.
 
@@ -72,7 +72,7 @@ Proof.
     eapply wf_exp_eq_conv' with {{{ ^ (iter (S (length Γ1)) (fun A1 : exp P => {{{ A1[Wk] }}}) A0)[Wk][τ] }}}; mauto 3.
 
     deepexec (@wf_ctx_sub_ctx_lookup P) ltac:(fun H => destruct H as [Γ1' [? [Γ2' [? [-> [? [-> []]]]]]]]).
-    repeat rewrite List.length_app in *.
+    repeat rewrite List.app_length in *.
     replace (length Γ1) with (length Γ1') in * by lia.
     clear_refl_eqs.
     replace (length Γ2) with (length Γ2') by (simpl in *; lia).
